Examples/CellSpec.v
@@ -1,0 +1,56 @@
+From LHL.Core Require Import
+  Program
+  Specs.
+
+Variant CellSig {A} : ESig :=
+| Write (x : A) : CellSig unit
+| Read : CellSig A.
+Arguments CellSig : clear implicits.
+
+Record CellPend {A} := MkCellPend {
+  CellThread : ThreadName;
+  CellRetTy : Type;
+  CellName : CellSig A CellRetTy
+}.
+Arguments CellPend : clear implicits.
+Arguments MkCellPend {A}.
+
+Variant CellState {A} :=
+| CellUB (* todo: make sequentially consistent *)
+| CellDef (v : option A) (m : option (CellPend A)).
+Arguments CellState : clear implicits.
+
+Definition CellUndef {A} := @CellDef A None None.
+Definition CellIdle {A} (v : option A) := CellDef v None.
+Definition CellWriteRan {A} i v (v' : A) :=
+  CellDef v (Some (MkCellPend i _ (Write v'))).
+Definition CellReadRan {A} i (v : A) :=
+  CellDef (Some v) (Some (MkCellPend i _ Read)).
+
+Variant CellStep {A} : CellState A -> ThreadEvent (CellSig A) -> CellState A -> Prop :=
+| CellCallWrite i v v' :
+    CellStep (CellIdle v) (i, CallEv (Write v')) (CellWriteRan i v v')
+| CellRetWrite i v v' :
+    CellStep (CellWriteRan i v v') (i, RetEv (Write v') tt) (CellIdle (Some v'))
+| CellCallRead i v :
+    CellStep (CellIdle (Some v)) (i, CallEv Read) (CellReadRan i v)
+| CellRetRead i v :
+    CellStep (CellReadRan i v) (i, RetEv Read v) (CellIdle (Some v))
+| CellDoubleWrite i j v v' v'' :
+    i <> j ->
+    CellStep (CellWriteRan i v v') (j, CallEv (Write v'')) CellUB
+| CellDoubleRead i j v :
+    i <> j ->
+    CellStep (CellReadRan i v) (j, CallEv Read) CellUB
+| CellReadUndef i :
+    CellStep (CellIdle None) (i, CallEv Read) CellUB
+| CellStepUB e :
+    CellStep CellUB e CellUB.
+
+Program Definition cellSpec A : Spec (CellSig A) := {|
+  State := CellState A;
+  Step := CellStep;
+  Init := CellUndef
+|}.
+
+Admit Obligations.
