Examples/Snapshot.v
@@ -1,0 +1,71 @@
+From LHL.Core Require Import
+  Program
+  ProgramRules
+  Specs
+  Logic
+  LogicFacts
+  Tensor
+  Traces
+  Linearizability.
+
+From LHL.Examples Require Import
+  CellSpec
+  ThreadLocal
+  WriteSnapshotSpec.
+
+From LHL.Util Require Import
+  Tactics
+  TransUtil
+  Util.
+
+From Coq Require Import
+  Strings.String.
+
+Definition Underlay A :=
+  LocalSig (CellSig A) |+| LocalSig (CellSig (set A * set A)) |+| LocalSig (CellSig nat).
+Definition VE A : Spec (Underlay A) :=
+  tensorSpec (localSpec (cellSpec _))(tensorSpec (localSpec (cellSpec _)) (localSpec (cellSpec _))).
+
+Definition bool_prop (P : Prop) : bool :=
+  if classicT P then true else false.
+
+(* fst is old, snd is new *)
+Definition query {n} {A} self : Prog (Underlay A) (set A) :=
+  call (At self (Write (emp, emp)));;
+  while (
+    sets <- call (At self Read);
+    ret (fst sets /=? snd sets)
+  ) (
+    call (At self (Write 0));;
+    (* get old *)
+    while (
+      i <- call (At self Read);
+      ret (bool_prop (i < n))
+    ) (
+      i <- call (At self Read);
+      v <- call (At i Read);
+      sets <- call (At self Read);
+      call (At self (Write (insert (fst sets) v, snd sets)))
+    );;
+    call (At self (Write 0));;
+    (* get new *)
+    while (
+      i <- call (At self Read);
+      ret (bool_prop (i < n))
+    ) (
+      i <- call (At self Read);
+      v <- call (At i Read);
+      sets <- call (At self Read);
+      call (At self (Write (fst sets, insert (snd sets) v)))
+    )
+  );;
+  sets <- call (At self Read);
+  ret (fst sets).
+
+Definition update {A} self (v : A) : Prog (Underlay A) unit :=
+  call (At self (Write v)).
+
+(* Definition snapshotImpl n A : Impl (Underlay A) (SnapshotSig A) :=
+  fun i m => match m with
+  | Update v => update v
+  end. *)
