Examples/SnapshotSpec.v
@@ -1,0 +1,55 @@
+From LHL.Core Require Import
+  Program
+  Specs.
+
+From LHL.Examples Require Import
+  OMemSpec.
+
+From LHL.Util Require Import
+  Util.
+
+Definition set A := A -> bool.
+
+Definition insert {A} (s : set A) (x : A) : set A :=
+  fun y => if x =? y then true else s y.
+
+Definition emp {A} : set A := fun _ => false.
+
+Variant SnapshotSig {A} : ESig :=
+| Update (v : A) : SnapshotSig unit
+| Query : SnapshotSig (set A).
+Arguments SnapshotSig : clear implicits.
+
+Variant SnapshotState {A} :=
+| SnapDef (vs : set A) (m : ThreadName -> option {B & SnapshotSig A B}).
+Arguments SnapshotState : clear implicits.
+
+Variant SnapshotStep {A} : SnapshotState A -> ThreadEvent (SnapshotSig A) -> SnapshotState A -> Prop :=
+| SnapCallUpdate i v vs m m' :
+    m i = None ->
+    m' i = Some (existT _ _ (Update v)) ->
+    differ_pointwise m m' i ->
+    SnapshotStep (SnapDef vs m) (i, CallEv (Update v)) (SnapDef vs m')
+| SnapRetUpdate i v vs m m' :
+    m i = Some (existT _ _ (Update v)) ->
+    m' i = None ->
+    differ_pointwise m m' i ->
+    SnapshotStep (SnapDef vs m) (i, RetEv (Update v) tt) (SnapDef (insert vs v) m')
+| SnapCallQuery i vs m m' :
+    m i = None ->
+    m' i = Some (existT _ _ Query) ->
+    differ_pointwise m m' i ->
+    SnapshotStep (SnapDef vs m) (i, CallEv Query) (SnapDef vs m')
+| SnapRetQuery i vs m m' :
+    m i = Some (existT _ _ Query) ->
+    m' i = None ->
+    differ_pointwise m m' i ->
+    SnapshotStep (SnapDef vs m) (i, RetEv Query vs) (SnapDef vs m').
+
+Program Definition snapshotSpec A : Spec (SnapshotSig A) := {|
+  State := SnapshotState A;
+  Step := SnapshotStep;
+  Init := SnapDef emp (fun _ => None)
+|}.
+
+Admit Obligations.
