Examples/ThreadLocal.v
@@ -1,0 +1,57 @@
+From LHL.Core Require Import
+  Program
+  ProgramRules
+  Specs
+  Logic
+  LogicFacts
+  Tensor
+  Traces
+  Linearizability.
+
+From LHL.Examples Require Import
+  OMemSpec
+  WriteSnapshotSpec.
+
+From LHL.Util Require Import
+  Tactics
+  TransUtil
+  Util.
+
+Fixpoint ESigN n E : ESig :=
+  match n with
+  | 0 => E
+  | S n => E |+| ESigN n E
+  end.
+
+Fixpoint tensorNSpec {E} n (V : Spec E) : Spec (ESigN n E) :=
+  match n with
+  | 0 => V
+  | S n => tensorSpec V (tensorNSpec n V)
+  end.
+
+Variant LocalSig {E : ESig} : ESig :=
+| At {A} (i : ThreadName) (m : E A) : LocalSig A.
+Arguments LocalSig : clear implicits.
+
+Variant LocalStep {E} {V : Spec E} : (ThreadName -> State V) -> ThreadEvent (LocalSig E) -> (ThreadName -> State V) -> Prop :=
+| LocalCall i A (m : E A) s x t y :
+    s i = x ->
+    t i = y ->
+    differ_pointwise s t i ->
+    V.(Step) x (i, CallEv m) y ->
+    LocalStep s (i, CallEv (At i m)) t
+| LocalRet i A (m : E A) v s x t y :
+    s i = x ->
+    t i = y ->
+    differ_pointwise s t i ->
+    V.(Step) x (i, RetEv m v) y ->
+    LocalStep s (i, RetEv (At i m) v) t.
+Arguments LocalStep {E} V.
+
+Program Definition localSpec {E} (V : Spec E) : Spec (LocalSig E) := {|
+  State := ThreadName -> State V;
+  Step := LocalStep V;
+  Init _ := Init V
+|}.
+
+Admit Obligations.
